Exercise 7

teaching/taltech2018/ex/ex7/BinarySearchTree.fst
@@ -48,28 +48,21 @@ private type btree =
 *)
 
 private let rec btree_contains (t:btree) (n:nat) : GTot bool =
-  match t with 
-  | Leaf -> false
-  | Node t1 m t2 -> 
-      if n = m then true else 
-      if n < m then t1 `btree_contains` n
-               else t2 `btree_contains` n
+  admit ()
 
 (* 
 
-  Task 1.2: Define empty binary trees and insertion into binary (search) trees.
+  Task 1.2: Define the empty binary tree and insertion into binary trees. For the latter, again assume as 
+            if you were working with binary **search** trees, i.e., insert the given value `n` so that if 
+            the given tree `t` happens to be a binary search tree, so will be the returned binary tree.
 
 *)
 
-private let empty_btree () : GTot btree = Leaf
+private let empty_btree () : GTot btree = 
+  admit ()
 
 private let rec btree_insert (t:btree) (n:nat) : GTot btree =
-  match t with 
-  | Leaf -> Node Leaf n Leaf
-  | Node t1 m t2 -> 
-      if n = m then Node t1 m t2 else
-      if n < m then Node (btree_insert t1 n) m t2
-               else Node t1 m (btree_insert t2 n)
+  admit ()
 
 (*
 
@@ -79,25 +72,8 @@ private let rec btree_insert (t:btree) (n:nat) : GTot btree =
 
 *)
 
-private let rec sorted_left_of (t:btree) (n:nat) : GTot bool = 
-  match t with
-  | Leaf -> true
-  | Node t1 m t2 -> t1 `sorted_left_of` m && 
-                    m < n && 
-                    t2 `sorted_right_of` m
-
-and sorted_right_of (t:btree) (n:nat) : GTot bool = 
-  match t with
-  | Leaf -> true
-  | Node t1 m t2 -> t1 `sorted_left_of` m && 
-                    m > n && 
-                    t2 `sorted_right_of` m
-
 private let rec sorted (t:btree) : GTot bool =
-  match t with
-  | Leaf -> true
-  | Node t1 n t2 -> t1 `sorted_left_of` n && 
-                    t2 `sorted_right_of` n
+  admit ()
 
 
 (** PART 2 **)
@@ -106,60 +82,6 @@ private let rec sorted (t:btree) : GTot bool =
 
 abstract type stree = t:btree{sorted t}
 
-(* Useful lemmas about sortedness and the tree operations defined above *)
-
-private let rec lemma_btree_insert_is_sorted (t:btree) (n:nat) 
-  : Lemma (requires (sorted t))
-          (ensures  (sorted (btree_insert t n))) = 
-  match t with
-  | Leaf -> ()
-  | Node t1 m t2 -> 
-      if n = m then () else
-      if n < m then lemma_btree_insert_is_sorted t1 n
-               else lemma_btree_insert_is_sorted t2 n
-
-private let rec lemma_btree_insert_contains (t:btree) (n:nat) 
-  : Lemma (requires (sorted t))
-          (ensures  ((btree_insert t n) `btree_contains` n)) =
-  match t with
-  | Leaf -> ()
-  | Node t1 m t2 -> 
-      if n = m then () else
-      if n < m then lemma_btree_insert_contains t1 n
-               else lemma_btree_insert_contains t2 n
-
-private let rec lemma_contains_btree_insert_equal (t:btree) (n:nat) 
-  : Lemma (requires (sorted t && t `btree_contains` n))
-          (ensures  (btree_insert t n = t)) = 
-  match t with
-  | Node t1 m t2 -> 
-      if n = m then () else 
-      if n < m then lemma_contains_btree_insert_equal t1 n
-               else lemma_contains_btree_insert_equal t2 n
-
-private let rec lemma_distinct_btree_insert_contains (t:btree) (n m:nat)
-  : Lemma (requires ((btree_insert t n) `btree_contains` m))
-          (ensures  (t `btree_contains` m \/ n = m)) = 
-  match t with 
-  | Leaf -> ()
-  | Node t1 k t2 -> 
-      if n = k then () else 
-      if n < k then (Classical.or_elim #((btree_insert t1 n) `btree_contains` m) 
-                                       #(not((btree_insert t1 n) `btree_contains` m)) 
-                                       #(fun _ -> (Node t1 k t2) `btree_contains` m \/ n = m) 
-                                       (fun _ -> lemma_distinct_btree_insert_contains t1 n m) 
-                                       (fun _ -> ()))
-               else (Classical.or_elim #((btree_insert t2 n) `btree_contains` m) 
-                                       #(not((btree_insert t2 n) `btree_contains` m)) 
-                                       #(fun _ -> (Node t1 k t2) `btree_contains` m \/ n = m) 
-                                       (fun _ -> lemma_distinct_btree_insert_contains t2 n m) 
-                                       (fun _ -> ()))
-
-private let lemma_distinct_btree_insert_not_contains (t:btree) (n m:nat)
-  : Lemma (requires (not (t `btree_contains` m) /\ n <> m))
-          (ensures  (not ((btree_insert t n) `btree_contains` m))) = 
-  Classical.move_requires (fun _ -> lemma_distinct_btree_insert_contains t n m) ()
-
 (*
 
   Task 2.1: Define search/containment, creation of empty trees, and insertion operations for binary search trees.
@@ -167,14 +89,13 @@ private let lemma_distinct_btree_insert_not_contains (t:btree) (n m:nat)
 *)
 
 let stree_contains (t:stree) (n:nat) : GTot bool =
-  btree_contains t n
+  admit ()
 
 let empty_stree () : GTot stree = 
-  empty_btree ()
+  admit ()
 
 let stree_insert (t:stree) (n:nat) : GTot stree = 
-  lemma_btree_insert_is_sorted t n; 
-  btree_insert t n
+  admit ()
 
 (*
 
@@ -184,20 +105,28 @@ let stree_insert (t:stree) (n:nat) : GTot stree =
 
 let rec lemma_insert_contains (t:stree) (n:nat) 
   : Lemma ((stree_insert t n) `stree_contains` n) =
-  lemma_btree_insert_contains t n
+  admit ()
 
 let rec lemma_contains_insert_equal (t:stree) (n:nat) 
   : Lemma (requires (t `stree_contains` n))
           (ensures  (stree_insert t n = t)) = 
-  lemma_contains_btree_insert_equal t n
+  admit ()
 
 let lemma_distinct_insert_not_contains (t:stree) (n m:nat)
   : Lemma (requires (not (t `stree_contains` m) /\ n <> m))
           (ensures  (not ((stree_insert t n) `stree_contains` m))) = 
-  lemma_distinct_btree_insert_not_contains t n m
+  admit ()
 
 
 (** PART 3 **)
+
+(*
+
+  Importing standard library modules to do with erased ghost code (see the note below) and 
+  stateful programming (heaps, the `ST` effect, etc). Hint: You will highly likely need to 
+  have a look at these libraries and use the functionality they provide in your solution.
+
+*)
 
 open FStar.Ghost
 open FStar.Heap
@@ -231,22 +160,8 @@ let mtree = treeptr
 
 *)
 
-let rec wf (r:mtree) (t:stree) (h:heap) : GTot (option (Set.set nat)) (decreases t) =
-  match t , StrongExcludedMiddle.strong_excluded_middle (h `contains` r) , sel h r with
-  | Leaf , true , None -> Some (only r)
-  | Node t1 n t2 , true , Some nd -> (
-      match (wf nd.left t1 h) , (n = nd.value) , (wf nd.right t2 h) with
-      | Some s1 , true , Some s2 -> (
-          match not (Set.mem (addr_of r) s1) , not (Set.mem (addr_of r) s2) , 
-                StrongExcludedMiddle.strong_excluded_middle (Set.disjoint s1 s2) with 
-          | true , true , true -> Some (Set.union (only r) (Set.union s1 s2))
-          | _ -> None
-        )
-      | _ -> None
-    )
-  | _ -> None
-
-let is_stree (r:mtree) (t:stree) (h:heap) : GTot bool = Some? (wf r t h)
+let is_stree (r:mtree) (t:stree) (h:heap) : GTot bool = 
+  admit ()
 
 (*
 
@@ -256,8 +171,8 @@ let is_stree (r:mtree) (t:stree) (h:heap) : GTot bool = Some? (wf r t h)
             Hint: You will need to strengthen the specification of `search` to verify `BinarySearchTreeClient`.
 
   Note: Here we follow a common pattern in verification of threading a ghost state through our programs, where 
-        the ghost state (here, `t:erased stree`) is the purely functional specification of our mutable stateful 
-        code. We have wrapped `stree` in `erased` to ensure that it cannot be used computationally relevantly 
+        the ghost state (`t:erased stree`) is the purely functional specification of our mutable stateful code.
+        We have wrapped `stree` in the `erased` type to ensure that it cannot be used computationally relevantly 
         in user code (in that sense, `erased` is similar to the `GTot` effect). You can find more about the 
         `erased` type in the standard library in `FStar.Ghost`, including operations that you will need to use.
 
@@ -265,18 +180,8 @@ let is_stree (r:mtree) (t:stree) (h:heap) : GTot bool = Some? (wf r t h)
 
 let rec search (t:erased stree) (r:mtree) (n:nat) 
   : ST bool (requires (fun h0 -> is_stree r (reveal t) h0))
-            (ensures  (fun h0 b h1 -> h0 == h1 /\ 
-                                      b = (reveal t) `stree_contains` n)) =
-  match !r with 
-  | None -> false
-  | Some nd -> 
-      if n = nd.value then true else 
-      if n < nd.value then (let t1 = hide (match (reveal t) with 
-                                           | Node t1 _ _ -> t1) in 
-                            search t1 nd.left n)
-                      else (let t2 = hide (match (reveal t) with 
-                                           | Node _ _ t2 -> t2) in
-                            search t2 nd.right n)
+            (ensures  (fun h0 b h1 -> b = (reveal t) `stree_contains` n)) =
+  admit ()
 
 (*
 
@@ -289,11 +194,8 @@ let rec search (t:erased stree) (r:mtree) (n:nat)
 let create () 
   : ST (erased stree * mtree) (requires (fun _ -> True))
                               (ensures  (fun h0 (t,r) h1 -> 
-                                 reveal t = empty_stree () /\
-                                 fresh r h0 h1 /\
-                                 modifies !{} h0 h1 /\
-                                 wf r (reveal t) h1 == Some (only r))) =
-  hide Leaf , alloc None
+                                 reveal t = empty_stree ())) =
+  admit ()
 
 (*
 
@@ -303,68 +205,14 @@ let create ()
 
 *)
 
-let rec lemma_disjoint_wf_unchanged (r:mtree) (t:stree) (s:Set.set nat) (h0 h1:heap)
-  : Lemma (requires (Some? (wf r t h0) /\ 
-                     Set.disjoint (Some?.v (wf r t h0)) s /\ 
-                     modifies s h0 h1))
-          (ensures  (wf r t h0 == wf r t h1)) (decreases t)
-          [SMTPat (wf r t h0); SMTPat (modifies s h0 h1)]= 
-  match t with
-  | Leaf -> ()
-  | Node t1 n t2 -> 
-      let (Some nd) = sel h0 r in 
-      lemma_disjoint_wf_unchanged nd.left t1 s h0 h1;
-      lemma_disjoint_wf_unchanged nd.right t2 s h0 h1
-
-let rec lemma_wf_addrs_in (r:mtree) (t:stree) (h:heap)
-  : Lemma (requires (Some? (wf r t h)))
-          (ensures  (forall r' . Set.mem r' (Some?.v (wf r t h)) ==> ~(addr_unused_in r' h))) 
-          (decreases t)
-          [SMTPat (wf r t h)] = 
-  match t with 
-  | Leaf -> ()
-  | Node t1 n t2 -> 
-      let (Some nd) = sel h r in
-      lemma_wf_addrs_in nd.left t1 h;
-      lemma_wf_addrs_in nd.right t2 h
-
 (* Insertion into a mutable binary search tree *)
-
-let fresh_extension (s0 s1:Set.set nat) (h:heap) = 
-  Set.subset s0 s1 /\
-  (forall r . (not (Set.mem r s0) /\ Set.mem r s1) ==> addr_unused_in r h)
 
 let rec insert (t:erased stree) (r:mtree) (n:nat) 
   : ST (erased stree) (requires (fun h0 -> is_stree r (reveal t) h0))
                       (ensures  (fun h0 t' h1 -> 
-                         reveal t' = stree_insert (reveal t) n /\
-                         is_stree r (reveal t') h1 /\ (
-                         let (Some s0) = wf r (reveal t) h0 in 
-                         let (Some s1) = wf r (reveal t') h1 in
-                         modifies s0 h0 h1 /\
-                         fresh_extension s0 s1 h0))) = 
-  recall r;
-  match !r with
-  | None -> (
-      let t1,r1 = create () in
-      let t2,r2 = create () in  
-      r := Some ({left = r1; value = n; right = r2});
-      hide (Node (reveal t1) n (reveal t2)))
-  | Some nd -> 
-      if n = nd.value then t else
-      if n < nd.value then (let t1 = hide (match (reveal t) with 
-                                           | Node t1 _ _ -> t1) in
-                            let t2 = hide (match (reveal t) with 
-                                           | Node _ _ t2 -> t2) in
-                            let t1' = insert t1 (nd.left) n in 
-                            hide (Node (reveal t1') nd.value (reveal t2)))
-                      else (let t1 = hide (match (reveal t) with 
-                                           | Node t1 _ _ -> t1) in
-                            let t2 = hide (match (reveal t) with 
-                                           | Node _ _ t2 -> t2) in
-                            let t2' = insert t2 (nd.right) n in 
-                            hide (Node (reveal t1) nd.value (reveal t2')))
-
+                         reveal t' = stree_insert (reveal t) n)) = 
+  admit ()
+  
 (** PART 4 **)
 
 (*
